src/Language/PlutusIR/Semantics/Dynamic/Bigstep/Examples/IfThenElse.v
@@ -10,25 +10,50 @@ Require Import Coq.Strings.String.
 Local Open Scope string_scope.
 
 
+Ltac invert_neutrals :=
+  match goal with
+  | H : neutral_value ?n ?t |- False =>
+      inversion H; clear H; subst; try invert_neutrals
+  | H : neutral ?t |- False =>
+      inversion H; clear H; subst; try invert_neutrals
+  end.
+
+Ltac decide_neutral :=
+  match goal with
+  | |- neutral ?nv =>
+      unfold neutral; econstructor; simpl; eauto; try decide_neutral
+  | |- neutral_value ?n ?nv =>
+      econstructor; simpl; eauto; try decide_neutral
+  | |- ?f <> ?f' =>
+      let Hcon := fresh "Hcon" in
+      try solve [intros Hcon; inversion Hcon]
+  | |- ~ neutral ?t =>
+      let Hcon := fresh "Hcon" in
+      try solve [intros Hcon; invert_neutrals]
+  | |- ~ is_error ?t =>
+      let Hcon := fresh "Hcon" in
+      try solve [intros Hcon; inversion Hcon]
+  end.
+
 Definition Ty_int : Ty := Ty_Builtin (Some (TypeIn DefaultUniInteger)).
 Definition int_and_int_to_int : Ty := Ty_Fun Ty_int (Ty_Fun Ty_int Ty_int).
 
 Example test_ifThenElse : forall x y, exists k,
   Apply (LamAbs x int_and_int_to_int (Apply (Apply (Var x) (constInt 17)) (constInt 3))) (Apply (TyInst (Apply (LamAbs y Ty_int (Builtin IfThenElse)) (constInt 666)) (Ty_Builtin (Some (TypeIn DefaultUniInteger)))) (Constant (Some (ValueOf DefaultUniBool true)))) =[k]=> constInt 17.
-Proof with eauto.
+Proof with (eauto with hintdb__eval_no_error || (try solve [decide_neutral])).
   unfold constInt.
   intros.
   eexists.
-  eapply E_Apply... { 
-    eapply E_IfCondition...
-    eapply E_IfTyInst...
-    eapply E_Apply...
-    intros Hcon.
-    inversion Hcon.
-  } {
-    intros Hcon.
-    inversion Hcon.
-  }
-  simpl.
-  rewrite eqb_refl...
+  eapply E_Apply...
+  - eapply E_NeutralApplyPartial...
+    + eapply E_NeutralTyInstPartial...
+      * eapply E_Apply...
+      * simpl...
+      * eapply E_NeutralTyInst...
+    + simpl...
+    + eapply E_NeutralApply...
+  - simpl...
+  - simpl. rewrite eqb_refl.
+    eapply E_NeutralApplyFull...
+    repeat econstructor...
 Qed.
