src/Language/PlutusIR/Semantics/Dynamic/BuiltinMeanings.v
@@ -250,6 +250,20 @@ Definition compute_defaultfun (t : Term) : option Term :=
       )
       (Constant (@Some _ DefaultUniByteString (ValueOf _ bs2)))
     ) => Datatypes.Some (constBool (to_Z bs1 >? to_Z bs2))
+  (** If-Then-Else *)
+  | (Apply  
+      (Apply
+        (Apply
+          (TyInst
+            (Builtin IfThenElse)
+            T
+          )
+          (Constant (@Some _ DefaultUniBool (ValueOf _ cond)))
+        )
+        thenBranch
+      )
+      elseBranch
+    ) => Datatypes.Some (if cond then thenBranch else elseBranch)
   (* String operations *)
   (* CharToString *)
   | (Apply
